theories/Prelude/Notations.v
@@ -3,6 +3,8 @@ Require Import PnV.Prelude.SfLib.
 Reserved Infix "==" (no associativity, at level 70).
 Reserved Infix "≡" (no associativity, at level 70).
 Reserved Infix "≈" (no associativity, at level 70).
+Reserved Infix "≅" (no associativity, at level 70).
+Reserved Infix "≃" (no associativity, at level 70).
 
 Reserved Infix "≠" (no associativity, at level 70).
 
@@ -17,7 +19,7 @@ Reserved Infix "≼" (no associativity, at level 70).
 Reserved Infix "≈ₜ" (no associativity, at level 70).
 Reserved Infix "≳ₜ" (no associativity, at level 70).
 Reserved Infix "≲ₜ" (no associativity, at level 70).
-Reserved Infix "≅ₜ" (no associativity, at level 70).
+Reserved Infix "≃ₜ" (no associativity, at level 70).
 
 Reserved Infix "≦ᵣ" (no associativity, at level 70).
 Reserved Infix "=ᵣ" (no associativity, at level 70).
